\section{Cosine Orthogonality Lemma}
\label{app:cos-orth-lemma}

For any nonzero $q,k\in\mathbb{R}^d$,
\begin{align}
q^{\!\top}\,\nabla_q\,\cos(q,k) \,=\, 0.
\end{align}

\noindent\textit{Proof.} Let
\begin{equation}
\begin{aligned}
\cos(q,k) = f(q) = \frac{u(q)}{v(q)}, \\
u(q)=q^{\!\top}k,\; v(q)=\|q\|\,\|k\|.
\end{aligned}
\end{equation}
By the quotient rule,
\begin{align}
\nabla_q f \,=\, \frac{v\,\nabla_q u - u\,\nabla_q v}{v^2}.
\end{align}
The terms are
\begin{align}
\nabla_q u \,=\, k, \qquad \nabla_q v \,=\, \frac{\|k\|}{\|q\|}\, q.
\end{align}
Substituting and simplifying,
\begin{equation}
\begin{aligned}
\nabla_q f 
&= \frac{\|q\|\,\|k\|\,k - (q^{\!\top}k)\,\frac{\|k\|}{\|q\|}\, q}{\bigl(\|q\|\,\|k\|\bigr)^2} \\
&= \frac{1}{\|q\|\,\|k\|}\Bigl(k - \frac{q^{\!\top}k}{\|q\|^2}\, q\Bigr).
\end{aligned}
\end{equation}
Thus
\begin{equation}
\begin{aligned}
q^{\!\top}\nabla_q f 
&= \frac{1}{\|q\|\,\|k\|}\Bigl(q^{\!\top}k - \frac{q^{\!\top}k}{\|q\|^2}\, q^{\!\top}q\Bigr) \\
&= \frac{1}{\|q\|\,\|k\|}\Bigl(q^{\!\top}k - \frac{q^{\!\top}k}{\|q\|^2}\, \|q\|^2\Bigr) \\
&= 0. \qquad
\end{aligned}
\end{equation}


